Test/VProg.v
@@ -6,15 +6,15 @@ Import SL.Tactics.
 
 
 Section Program.
-  Variables (SIG : sig_context) (SPEC : CP.spec_context SIG).
+  Variable (CT : CP.context).
 
 
 Definition spec_0 : FDecl (ptr * ptr) _ unit _
   FOR (p0, p1)
   FOR (n0, n1) [] [vptr p0 ~> n0; vptr p1 ~> n1] True
   RET _ FOR tt [vptr p0 ~> n1; vptr p1 ~> n0] True.
-Proof. Derive. Defined.
-Variable f_0 : spec_0 _ SPEC.
+Proof. Derived. Defined.
+Variable f_0 : spec_0 CT.
 
 Definition vprog_0 : FImpl f_0 := fun '(p0, p1) =>
   'v0 <- Read p0;
@@ -23,23 +23,19 @@ Definition vprog_0 : FImpl f_0 := fun '(p0, p1) =>
   Write p1 v0.
 Lemma correct_0 : FCorrect vprog_0.
 Proof. by_wlp. Qed.
-Definition cp_0: f_extract vprog_0.
-Proof. Derive. Defined.
 
 
 Definition spec_1 : FDecl (ptr * ptr * ptr) _ unit _
   FOR (p0, p1, p2)
   FOR (n0, n1, n2) [vptr p2 ~> n2] [vptr p0 ~> n0; vptr p1 ~> n1] True
   RET _ FOR tt [vptr p0 ~> n1; vptr p1 ~> n0] True.
-Proof. Derive. Defined.
-Variable f_1 : spec_1 _ SPEC.
+Proof. Derived. Defined.
+Variable f_1 : spec_1 CT.
 
 Definition vprog_1 : FImpl f_1 := fun '(p0, p1, p2) =>
   f_0 (p0, p1).
 Lemma correct_1 : FCorrect vprog_1.
 Proof. by_wlp. Qed.
-Definition cp_1: f_extract vprog_1.
-Proof. Derive. Defined.
 
 
 Definition data42 : nat := 42.
@@ -48,8 +44,8 @@ Definition spec_2 : FDecl (ptr * ptr * ptr) _ ptr _
   FOR (p0, p1, p2)
   FOR (n0, n1, n2) [vptr p2 ~> n2] [vptr p0 ~> n0; vptr p1 ~> n1] True
   RET p FOR (n, n1') [vptr p ~> n; vptr p1 ~> n1'] (n1' > 0).
-Proof. Derive. Defined.
-Variable f_2 : spec_2 _ SPEC.
+Proof. Derived. Defined.
+Variable f_2 : spec_2 CT.
 
 Definition vprog_2 : FImpl f_2 := fun '(p0, p1, p2) =>
   'v0 <- Read p0;
@@ -62,39 +58,33 @@ Proof.
   by_wlp.
   unfold data42; repeat constructor.
 Qed.
-Definition cp_2: f_extract vprog_2.
-Proof. Derive. Defined.
 
 
 Definition spec_3 : FDecl ptr (Some (fun _ => ptr)) ptr (Some (fun _ => ptr))
   FOR p0 & p1
   FOR (n0, n1) [] [vptr p0 ~> n0; vptr p1 ~> n1] True
   RET p0' & p1' FOR (n0', n1') [vptr p0' ~> n0'; vptr p1' ~> n1'] True.
-Proof. Derive. Defined.
-Variable f_3 : spec_3 _ SPEC.
+Proof. Derived. Defined.
+Variable f_3 : spec_3 CT.
 
 Definition vprog_3 : FImpl f_3 := fun p0 p1 =>
   RetG p0 p1 (pt := fun p0 p1 => [vptr p0 ~>; vptr p1 ~>]).
 Lemma correct_3: FCorrect vprog_3.
 Proof. by_wlp. Qed.
-Definition cp_3: f_extract vprog_3.
-Proof. Derive. Defined.
 
 
 Definition spec_4 : FDecl (ptr * ptr) _ ptr (Some (fun _ => ptr))
   FOR (p0, p1)
   FOR (n0, n1) [] [vptr p0 ~> n0; vptr p1 ~> n1] True
   RET p0' & p1' FOR (n0', n1') [vptr p0' ~> n0'; vptr p1' ~> n1'] True.
-Proof. Derive. Defined.
-Variable f_4 : spec_4 _ SPEC.
+Proof. Derived. Defined.
+Variable f_4 : spec_4 CT.
 
 Definition vprog_4 : FImpl f_4 := fun '(p0, p1) =>
   'p0' p1' <- f_3 p0 p1;
   RetG p0' p1' (pt := fun p0 p1 => [vptr p0 ~>; vptr p1 ~>]).
 Lemma correct_4: FCorrect vprog_4.
 Proof. by_wlp. Qed.
-Definition cp_4: f_extract vprog_4.
-Proof. Derive. Defined.
 
 
 Definition cell2 (p : ptr) '(v0, v1) : SLprop.t :=
@@ -103,7 +93,7 @@ Definition cell2 (p : ptr) '(v0, v1) : SLprop.t :=
 Definition elim_cell2_spec : LDecl ptr unit
   FOR p FOR n01 [] [cell2 p ~> n01] True
   RET _ FOR tt [vptr p ~> (fst n01); vptr (S p) ~> (snd n01)] True.
-Proof. Derive. Defined.
+Proof. Derived. Defined.
 Lemma elim_cell2 : elim_cell2_spec.
 Proof.
   init_lemma p (n0, n1) _.
@@ -113,24 +103,19 @@ Qed.
 Definition intro_cell2_spec : LDecl ptr unit
   FOR p FOR (n0, n1) [] [vptr p ~> n0; vptr (S p) ~> n1] True
   RET _ FOR tt [cell2 p ~> (n0, n1)] True.
-Proof. Derive. Defined.
+Proof. Derived. Defined.
 Lemma intro_cell2 : intro_cell2_spec.
 Proof.
   init_lemma p (n0, n1) _.
   reflexivity.
 Qed.
 
-(*
-Global Opaque cell2.
-Global Arguments cell2 : simpl never.
-*)
-
 Definition spec_5 : FDecl ptr _ unit _
   FOR p
   FOR v [] [cell2 p ~> v] True
   RET _ FOR v' [cell2 p ~> v'] (v' = let (n0, n1) := v in (S n0, n1)).
-Proof. Derive. Defined.
-Variable f_5 : spec_5 _ SPEC.
+Proof. Derived. Defined.
+Variable f_5 : spec_5 CT.
 
 Definition vprog_5 : FImpl f_5 := fun p =>
   gLem elim_cell2 p;;
@@ -139,76 +124,21 @@ Definition vprog_5 : FImpl f_5 := fun p =>
   gLem intro_cell2 p.
 Lemma correct_5: FCorrect vprog_5.
 Proof. by_wlp. case sel0; reflexivity. Qed.
-Definition cp_5: f_extract vprog_5.
-Proof. Derive. Defined.
 
 End Program.
 
-Section Extraction.
-  Definition SIG : sig_context :=
-    fun f => match f with
-    | 0 => Some (fd_sig spec_0)
-    | 1 => Some (fd_sig spec_1)
-    | 2 => Some (fd_sig spec_2)
-    | 3 => Some (fd_sig spec_3)
-    | 4 => Some (fd_sig spec_4)
-    | 5 => Some (fd_sig spec_5)
-    | _ => None
-    end.
-
-  Definition SPEC : CP.spec_context SIG :=
-    fun f => match f with
-    | 0 => fd_cp spec_0
-    | 1 => fd_cp spec_1
-    | 2 => fd_cp spec_2
-    | 3 => fd_cp spec_3
-    | 4 => fd_cp spec_4
-    | 5 => fd_cp spec_5
-    | _ => tt
-    end.
-
-  Definition H_f_0 := fd_mk 0 spec_0 SPEC eq_refl eq_refl.
-  Definition H_f_1 := fd_mk 1 spec_1 SPEC eq_refl eq_refl.
-  Definition H_f_2 := fd_mk 2 spec_2 SPEC eq_refl eq_refl.
-  Definition H_f_3 := fd_mk 3 spec_3 SPEC eq_refl eq_refl.
-  Definition H_f_4 := fd_mk 4 spec_4 SPEC eq_refl eq_refl.
-  Definition H_f_5 := fd_mk 5 spec_5 SPEC eq_refl eq_refl.
-
-  Definition IMPL : CP.impl_context SIG :=
-    fun f => match f with
-    | 0 => proj1_sig (cp_0 _ _ H_f_0)
-    | 1 => proj1_sig (cp_1 _ _ H_f_0 H_f_1)
-    | 2 => proj1_sig (cp_2 _ _ H_f_2)
-    | 3 => proj1_sig (cp_3 _ _ H_f_3)
-    | 4 => proj1_sig (cp_4 _ _ H_f_3 H_f_4)
-    | 5 => proj1_sig (cp_5 _ _ H_f_5)
-    | _ => tt
-    end.
-
-  Lemma match_context:
-    CP.context_match_spec IMPL SPEC.
-  Proof.
-    Tac.case_until_True;
-    cbn beta iota delta [SIG IMPL SPEC];
-    apply f_extract_match_spec.
-    - apply correct_0.
-    - apply correct_1.
-    - apply correct_2.
-    - apply correct_3.
-    - apply correct_4.
-    - apply correct_5.
-  Qed.
-
-  Lemma context_oracle_free:
-    CP.context_oracle_free IMPL.
-  Proof.
-    Tac.case_until_True;
-    cbn beta iota delta [SIG IMPL SPEC];
-    apply f_extract_oracle_free.
-  Qed.
-End Extraction.
+Derive prog SuchThat (CP.of_entries [
+  f_entry spec_0 correct_0;
+  f_entry spec_1 correct_1;
+  f_entry spec_2 correct_2;
+  f_entry spec_3 correct_3;
+  f_entry spec_4 correct_4;
+  f_entry spec_5 correct_5
+] prog) As prog_correct.
+Proof. Derived. Qed.
 
 Section Other.
+  Variable CT : ConcreteProg.context.
 
 Definition sigh_a0 := mk_f_sig1 (ptr * ptr) None unit None.
 Definition spec_a0 : FSpec sigh_a0
@@ -217,7 +147,7 @@ Definition spec_a0 : FSpec sigh_a0
   RET _ FOR tt [] True.
 Proof. Tac.build_FSpec. Defined.
 
-Definition vprog_a0 : f_body SPEC sigh_a0 := fun ps =>
+Definition vprog_a0 : f_body CT sigh_a0 := fun ps =>
   'v0 <- let (p0, _) := ps in Read p0;
   Ret tt.
 Lemma imatch_a0:
@@ -235,7 +165,7 @@ Definition spec_a1a : FSpec sigh_a1a
   RET _ FOR (n1', n2') [vptr p1 ~> n1'; vptr p2 ~> n2'] (b = true -> n1' = 0).
 Proof. Tac.build_FSpec. Defined.
 
-Definition vprog_a1a : f_body SPEC sigh_a1a := fun '(b, p0, p1, p2) =>
+Definition vprog_a1a : f_body CT sigh_a1a := fun '(b, p0, p1, p2) =>
   if b
   then Write p1 0
   else Write p2 1.
@@ -256,7 +186,7 @@ Definition spec_a1b : FSpec sigh_a1b
   RET _ FOR n' [vptr p ~> n'] (b <> B1 -> n' = 0).
 Proof. Tac.build_FSpec. Defined.
 
-Definition vprog_a1b : f_body SPEC sigh_a1b := fun '(b, p) =>
+Definition vprog_a1b : f_body CT sigh_a1b := fun '(b, p) =>
   match b with
   | B0 => Write p 0
   | B1 | B2 => Ret tt
@@ -273,7 +203,7 @@ Definition spec_a1c : FSpec sigh_a1c
   RET _ FOR n' [vptr p ~> n'] (n' > 0).
 Proof. Tac.build_FSpec. Defined.
 
-Definition vprog_a1c : f_body SPEC sigh_a1c := fun '(o, p) =>
+Definition vprog_a1c : f_body CT sigh_a1c := fun '(o, p) =>
   match o with
   | Some n => Write p n
   | None   => Ret tt
@@ -290,7 +220,7 @@ Definition spec_a2a : FSpec sigh_a2a
   RET _ FOR n1' [vptr p1 ~> n1'] (n0 <= n1').
 Proof. Tac.build_FSpec. Defined.
 
-Definition vprog_a2a : f_body SPEC sigh_a2a := fun '(p0, p1) =>
+Definition vprog_a2a : f_body CT sigh_a2a := fun '(p0, p1) =>
   'v1 <- Read p1;
   'v0 <- gGet (SLprop.cell p0);
   Assert (fun 'tt => ([], v0 <= v1));;
@@ -301,7 +231,7 @@ Proof. by_wlp. Qed.
 Definition cp_a2a: f_extract vprog_a2a.
 Proof. Tac.extract_impl. Defined.
 
-Definition vprog_a2b : f_body SPEC sigh_a2a := fun '(p0, p1) =>
+Definition vprog_a2b : f_body CT sigh_a2a := fun '(p0, p1) =>
   'v1 v0 <- (
     'v1 <- Read p1;
     'v0 <- gGet (SLprop.cell p0);
@@ -322,7 +252,7 @@ Definition spec_a3 : FSpec sigh_a3
   RET _ & r FOR tt [] (r = n0 + n1).
 Proof. Tac.build_FSpec. Defined.
 
-Definition vprog_a3 : f_body SPEC sigh_a3 := fun _ '(n0, n1) =>
+Definition vprog_a3 : f_body CT sigh_a3 := fun _ '(n0, n1) =>
   RetG tt (n0 + n1).
 Lemma imatch_a3:
   f_body_match vprog_a3 (m_spec spec_a3).
