VProg/Main.v
@@ -1,4 +1,11 @@
 From SLFun.VProg Require Export Vprop Core Ghost.
 
-Module Tactics   := Core.Tactics.
-Module Notations := Core.Notations.
+Module Tactics.
+  Export ConcreteProg.Tactics.
+  Export VProg.Core.Tactics.
+End Tactics.
+
+Module Notations.
+  Export Tactics.
+  Export VProg.Core.Notations.
+End Notations.
